src/3d/Binding.fsti
@@ -36,6 +36,7 @@ val bind_decls (g:global_env) (p:list decl) : ML (list decl & global_env)
 val initial_global_env (_:unit) : ML global_env
 val get_exported_decls (ge:global_env) (mname:string) : ML (list ident' & list ident')  //exported, private
 
+val is_output_type_ident (ge:global_env) (id:ident) : ML bool
 val get_output_exprs (ge:global_env) : ML (list (out_expr & bool))
 
 val finish_module (ge:global_env) (mname:string) (e_and_p:list ident' & list ident')
